src/lib/extraction/ListDef.ml
@@ -23,3 +23,25 @@ let rec repeat x n =
     (fun _ -> [])
     (fun k -> x :: (repeat x k))
     n
+
+(** val firstn : Big_int_Z.big_int -> 'a1 list -> 'a1 list **)
+
+let rec firstn n l =
+  (fun fO fS n -> if Big_int_Z.sign_big_int n <= 0 then fO ()
+  else fS (Big_int_Z.pred_big_int n))
+    (fun _ -> [])
+    (fun n0 -> match l with
+               | [] -> []
+               | a :: l0 -> a :: (firstn n0 l0))
+    n
+
+(** val skipn : Big_int_Z.big_int -> 'a1 list -> 'a1 list **)
+
+let rec skipn n l =
+  (fun fO fS n -> if Big_int_Z.sign_big_int n <= 0 then fO ()
+  else fS (Big_int_Z.pred_big_int n))
+    (fun _ -> l)
+    (fun n0 -> match l with
+               | [] -> []
+               | _ :: l0 -> skipn n0 l0)
+    n
