src/lib/extraction/list_basics.ml
@@ -1,6 +1,15 @@
 
 module Coq_list =
  struct
+  (** val replicate : Big_int_Z.big_int -> 'a1 -> 'a1 list **)
+
+  let rec replicate n x =
+    (fun fO fS n -> if Big_int_Z.sign_big_int n <= 0 then fO ()
+  else fS (Big_int_Z.pred_big_int n))
+      (fun _ -> [])
+      (fun n0 -> x :: (replicate n0 x))
+      n
+
   (** val foldl : ('a1 -> 'a2 -> 'a1) -> 'a1 -> 'a2 list -> 'a1 **)
 
   let rec foldl f a = function
