src/rocq/lib/Domain/TransferBitvectorInterval.v
@@ -1,0 +1,628 @@
+(* ************************************************************************ *)
+(*  Sail and the Sail architecture models here, comprising all files and    *)
+(*  directories except the ASL-derived Sail code in the aarch64 directory,  *)
+(*  are subject to the BSD two-clause licence below.                        *)
+(*                                                                          *)
+(*  The ASL derived parts of the ARMv8.3 specification in                   *)
+(*  aarch64/no_vector and aarch64/full are copyright ARM Ltd.               *)
+(*                                                                          *)
+(*  Copyright (c) 2013-2026                                                 *)
+(*    Kathyrn Gray                                                          *)
+(*    Shaked Flur                                                           *)
+(*    Stephen Kell                                                          *)
+(*    Gabriel Kerneis                                                       *)
+(*    Robert Norton-Wright                                                  *)
+(*    Christopher Pulte                                                     *)
+(*    Peter Sewell                                                          *)
+(*    Alasdair Armstrong                                                    *)
+(*    Brian Campbell                                                        *)
+(*    Thomas Bauereiss                                                      *)
+(*    Anthony Fox                                                           *)
+(*    Jon French                                                            *)
+(*    Dominic Mulligan                                                      *)
+(*    Stephen Kell                                                          *)
+(*    Mark Wassell                                                          *)
+(*    Alastair Reid (Arm Ltd)                                               *)
+(*                                                                          *)
+(*  All rights reserved.                                                    *)
+(*                                                                          *)
+(*  This work was partially supported by EPSRC grant EP/K008528/1 REMS:     *)
+(*  Rigorous Engineering for Mainstream Systems, an ARM iCASE award, EPSRC  *)
+(*  IAA KTF funding, and donations from Arm. This project has received      *)
+(*  funding from the European Research Council (ERC) under the European     *)
+(*  Union's Horizon 2020 research and innovation programme (grant agreement *)
+(*  No 789108, ELVER).                                                      *)
+(*                                                                          *)
+(*  This software was developed by SRI International and the University of  *)
+(*  Cambridge Computer Laboratory (Department of Computer Science and       *)
+(*  Technology) under DARPA/AFRL contracts FA8650-18-C-7809 ("CIFV")        *)
+(*  and FA8750-10-C-0237 ("CTSRD").                                         *)
+(*                                                                          *)
+(*  SPDX-License-Identifier: BSD-2-Clause                                   *)
+(* ************************************************************************ *)
+
+From Stdlib Require Import Logic.ProofIrrelevance.
+From Stdlib Require Import ZArith.
+
+From stdpp Require Import base.
+From stdpp Require Import gmap.
+From stdpp Require Import bitvector.definitions.
+From stdpp Require Import bitvector.tactics.
+
+From Sail Require Import Domain.Lattice.
+From Sail.Domain Require AbsBitvector.
+From Sail.Domain Require Interval.
+From Sail Require Bit.
+From Sail Require Import BvUtil.
+
+Import Bit.Three.
+
+Module B := AbsBitvector.Dom.
+Module I := Interval.Dom.
+
+Module BP := DomainProperties AbsBitvector.Bits B.
+
+Module Ops <: SAIL_BITS_INT B I.
+
+  Definition nonneg_top : I.t :=
+    I.Ends (exist _ (Some 0%Z, None) (I.low_high_plus_inf 0%Z)).
+
+  (* Minimum unsigned value of abstract bits (LSB-first), `pow` is the weight of the first bit *)
+  Fixpoint unsigned_lo (bits : list ubit) (pow : Z) : Z :=
+    match bits with
+    | []         => 0%Z
+    | B0 :: rest => unsigned_lo rest (2 * pow)%Z
+    | B1 :: rest => (pow + unsigned_lo rest (2 * pow))%Z
+    | BU :: rest => unsigned_lo rest (2 * pow)%Z
+    end.
+
+  (* Maximum unsigned value of abstract bits (LSB-first) *)
+  Fixpoint unsigned_hi (bits : list ubit) (pow : Z) : Z :=
+    match bits with
+    | []         => 0%Z
+    | B0 :: rest => unsigned_hi rest (2 * pow)%Z
+    | B1 :: rest => (pow + unsigned_hi rest (2 * pow))%Z
+    | BU :: rest => (pow + unsigned_hi rest (2 * pow))%Z
+    end.
+
+  Definition bits_unsigned_interval (bits : list ubit) : I.t :=
+    I.join (I.α (unsigned_lo bits 1%Z)) (I.α (unsigned_hi bits 1%Z)).
+
+  (* For each width in the abstract bitvector map, compute and join unsigned intervals *)
+  Definition unsigned (x : B.t) : I.t :=
+    match x with
+    | B.Top   => nonneg_top
+    | B.Bvs m =>
+        map_fold (λ (_ : nat) bits acc,
+          I.join (bits_unsigned_interval bits) acc) I.bot (`m)
+    end.
+
+  Lemma I_join_idem : ∀ x : I.t, I.join x x = x.
+  Proof.
+    intros x.
+    rewrite <- (I.meet_id x) at 2.
+    apply I.absorption_join_meet.
+  Qed.
+
+  Lemma concrete_lo_eq_hi : ∀ (bs : list bool) (pow : Z),
+    unsigned_lo (List.map from_bool bs) pow = unsigned_hi (List.map from_bool bs) pow.
+  Proof.
+    intros bs.
+    induction bs as [| b bs IH]; intros pow.
+    - reflexivity.
+    - destruct b; cbn; rewrite IH; reflexivity.
+  Qed.
+
+  Lemma unsigned_lo_spec : ∀ (bs : list bool) (pow : Z),
+    (0 ≤ pow)%Z →
+    (unsigned_lo (List.map from_bool bs) pow =
+     pow * BoolList.to_Z_unsigned (rev bs) None)%Z.
+  Proof.
+    induction bs as [| b bs IH]; intros pow Hpow.
+    - cbn. lia.
+    - cbn [List.map rev List.app].
+      rewrite BoolList.to_Z_unsigned_app, BoolList.Z_shiftl_1, BoolList.Z_lor_even;
+        [| apply BoolList.to_Z_unsigned_nonneg].
+      specialize (IH (2 * pow)%Z ltac:(lia)).
+      destruct b; cbn; rewrite IH; lia.
+  Qed.
+
+  Lemma bv_unsigned_to_Z : ∀ {n} (x : bv n),
+    bv_unsigned x = BoolList.to_Z_unsigned (rev (bv_to_bits x)) None.
+  Proof.
+    intros n x.
+    pose proof (BoolList.to_bv_ex x) as [y [Hlen Heq]].
+    specialize (Heq Hlen).
+    assert (Hbits : bv_to_bits x = rev y).
+    { rewrite Heq, bv_cast_bits. apply BoolList.bv_round_trip_alt. }
+    rewrite Hbits, rev_involutive.
+    rewrite Heq, bv_cast_unsigned.
+    apply BoolList.to_bv_unsigned.
+  Qed.
+
+  Lemma unsigned_abst : ∀ {n} {x : bv n},
+    I.α (bv_unsigned x) = unsigned (B.α (bv_to_bvn x)).
+  Proof.
+    intros n x.
+    rewrite B.abstract_bvs.
+    unfold unsigned, bits_unsigned_interval.
+    cbn [proj1_sig].
+    rewrite map_fold_singleton, I.join_id.
+    rewrite <- concrete_lo_eq_hi, I_join_idem.
+    f_equal.
+    rewrite unsigned_lo_spec; [| lia].
+    rewrite Z.mul_1_l.
+    exact (bv_unsigned_to_Z x).
+  Qed.
+
+  (* Signed interval from abstract bits: sign bit (MSB) contributes -2^(n-1) instead of +2^(n-1) *)
+  Definition bits_signed_interval (bits : list ubit) : I.t :=
+    match rev bits with
+    | [] => I.α 0%Z
+    | sign :: lower_rev =>
+        let lower := rev lower_rev in
+        let lo    := unsigned_lo lower 1%Z in
+        let hi    := unsigned_hi lower 1%Z in
+        let half  := (2 ^ Z.of_nat (length lower))%Z in
+        match sign with
+        | B0 => I.join (I.α lo) (I.α hi)
+        | B1 => I.join (I.α (lo - half)%Z) (I.α (hi - half)%Z)
+        | BU => I.join (I.α (lo - half)%Z) (I.α hi)
+        end
+    end.
+
+  Definition signed (x : B.t) : I.t :=
+    match x with
+    | B.Top   => I.top
+    | B.Bvs m =>
+        map_fold (λ (_ : nat) bits acc,
+          I.join (bits_signed_interval bits) acc) I.bot (`m)
+    end.
+
+  Lemma to_Z_unsigned_cons_None : ∀ (b : bool) (bs : list bool),
+    (BoolList.to_Z_unsigned (b :: bs) None =
+     bool_to_Z b * 2 ^ Z.of_nat (length bs) + BoolList.to_Z_unsigned bs None)%Z.
+  Proof.
+    intros b bs.
+    rewrite BoolList.to_Z_unsigned_cons, BoolList.to_Z_unsigned_split.
+    rewrite BoolList.lsb_prefix_to_Z.
+    cbn [BoolList.prefix_to_Z].
+    rewrite Z.shiftl_0_l, Z.add_0_l.
+    rewrite Z.shiftl_mul_pow2; [reflexivity | lia].
+  Qed.
+
+  Lemma unsigned_lo_concrete_rev : ∀ (bs : list bool),
+    (unsigned_lo (List.map from_bool (rev bs)) 1%Z = BoolList.to_Z_unsigned bs None)%Z.
+  Proof.
+    intros bs.
+    rewrite unsigned_lo_spec; [| lia].
+    rewrite Z.mul_1_l, rev_involutive.
+    reflexivity.
+  Qed.
+
+  Lemma bv_swrap_sign : ∀ (n : N) (s : bool) (lo : Z),
+    n ≠ 0%N →
+    (0 ≤ lo)%Z → (lo < bv_half_modulus n)%Z →
+    bv_swrap n (bool_to_Z s * bv_half_modulus n + lo)%Z =
+    (lo - bool_to_Z s * bv_half_modulus n)%Z.
+  Proof.
+    intros n s lo Hn Hlo_nn Hlo_lt.
+    pose proof (bv_half_modulus_twice n Hn) as Htwice.
+    pose proof (bv_half_modulus_nonneg n) as Hhalf_nn.
+    pose proof (bv_modulus_pos n) as Hmod_pos.
+    unfold bv_swrap, bv_wrap.
+    destruct s; cbn [bool_to_Z].
+    - replace (1 * bv_half_modulus n + lo + bv_half_modulus n)%Z
+        with (lo + 1 * bv_modulus n)%Z by lia.
+      rewrite Z.mod_add; [| lia].
+      rewrite Z.mod_small; lia.
+    - replace (0 * bv_half_modulus n + lo + bv_half_modulus n)%Z
+        with (lo + bv_half_modulus n)%Z by lia.
+      rewrite Z.mod_small; lia.
+  Qed.
+
+  Lemma signed_abst : ∀ {n} {x : bv n},
+    I.α (bv_signed x) = signed (B.α (bv_to_bvn x)).
+  Proof.
+    intros n x.
+    rewrite B.abstract_bvs.
+    unfold signed.
+    cbn [proj1_sig].
+    rewrite map_fold_singleton, I.join_id.
+    destruct (decide (n = 0%N)) as [-> | Hn].
+    - rewrite (bv_empty_canonical x), bv_empty_bits.
+      cbn. rewrite bv_signed_N_0. reflexivity.
+    - unfold bits_signed_interval.
+      rewrite <- map_rev.
+      assert (Hlen : length (rev (bv_to_bits x)) = N.to_nat n).
+      { rewrite length_rev. apply length_bv_to_bits. }
+      destruct (rev (bv_to_bits x)) as [| sign rest] eqn : Hrev.
+      + exfalso.
+        cbn in Hlen.
+        destruct n; [exact (Hn eq_refl) | lia].
+      + set (k := length rest).
+        assert (Hk : S k = N.to_nat n).
+        { cbn in Hlen. unfold k. exact Hlen. }
+        assert (Hn_eq : n = N.of_nat (S k)).
+        { symmetry. rewrite Hk. apply N2Nat.id. }
+        set (lo := BoolList.to_Z_unsigned rest None).
+        assert (Hunsigned : bv_unsigned x = (bool_to_Z sign * 2 ^ Z.of_nat k + lo)%Z).
+        { unfold lo.
+          rewrite bv_unsigned_to_Z, Hrev.
+          apply to_Z_unsigned_cons_None. }
+        assert (Hlo_nn : (0 ≤ lo)%Z) by apply BoolList.to_Z_unsigned_nonneg.
+        assert (Hhalf_eq : bv_half_modulus n = (2 ^ Z.of_nat k)%Z).
+        { pose proof (bv_half_modulus_twice n Hn) as Htwice.
+          unfold bv_modulus in Htwice.
+          rewrite Hn_eq, nat_N_Z, Nat2Z.inj_succ, Z.pow_succ_r in Htwice; [| lia].
+          rewrite Hn_eq. lia. }
+        assert (Hlo_lt : (lo < bv_half_modulus n)%Z).
+        { rewrite Hhalf_eq.
+          unfold lo.
+          pose proof (@BoolList.to_Z_unsiged_bv_modulus rest None) as H.
+          cbn [BoolList.prefix_size] in H. rewrite Nat.add_0_l in H.
+          unfold bv_modulus in H. rewrite nat_N_Z in H.
+          exact H. }
+        assert (Hsigned : bv_signed x = (lo - bool_to_Z sign * 2 ^ Z.of_nat k)%Z).
+        { unfold bv_signed.
+          rewrite Hunsigned, <- Hhalf_eq.
+          apply bv_swrap_sign; [exact Hn | exact Hlo_nn | exact Hlo_lt]. }
+        cbn [List.map].
+        rewrite <- map_rev.
+        assert (Hlo_eq : unsigned_lo (List.map from_bool (rev rest)) 1%Z = lo).
+        { unfold lo. apply unsigned_lo_concrete_rev. }
+        assert (Hhi_eq : unsigned_hi (List.map from_bool (rev rest)) 1%Z = lo).
+        { rewrite <- (concrete_lo_eq_hi (rev rest) 1). exact Hlo_eq. }
+        rewrite Hlo_eq, Hhi_eq.
+        assert (Hlen_k : length (List.map from_bool (rev rest)) = k).
+        { rewrite length_map, length_rev. reflexivity. }
+        rewrite Hlen_k, Hsigned.
+        destruct sign; cbn [from_bool bool_to_Z]; rewrite I_join_idem; f_equal; lia.
+  Qed.
+
+  Definition zeros_nat (n : nat) : B.t := B.α (bv_0 (N.of_nat n)).
+
+  Definition ones_nat (n : nat) : B.t := B.α (bv_not (bv_0 (N.of_nat n))).
+
+  (** This function intersects an interval with <<[0,∞)>>, converting
+      the resulting endpoints to natural numbers. Returns [None] if
+      the resulting interval is empty. For the upper bound, [None]
+      represents <<∞>>. *)
+  Definition nonneg_range (n : I.t) : option (nat * option nat) :=
+    match n with
+    | I.Empty => None
+    | I.Ends endpoints =>
+       match proj1_sig endpoints with
+       | (None, None) => Some (0, None)
+       | (Some lo, None) => Some (Z.to_nat lo, None)
+       | (None, Some hi) =>
+           if (hi <? 0)%Z then None else Some (0, Some (Z.to_nat hi))
+       | (Some lo, Some hi) =>
+           if (hi <? 0)%Z then None else Some (Z.to_nat lo, Some (Z.to_nat hi))
+       end
+    end.
+
+  Definition zeros (h : nat) (n : I.t) : B.t :=
+    match nonneg_range n with
+    | None => B.bot
+    | Some (_, None) => B.top
+    | Some (lo, Some hi) =>
+        let widths := hi - lo in
+        if h <=? widths then
+          B.top
+        else
+          fold_left (fun b w => B.join b (zeros_nat w)) (seq lo (hi - lo)) (zeros_nat hi)
+    end.
+
+  Lemma N_to_nat_via_Z : ∀ n, Z.to_nat (Z.of_N n) = N.to_nat n.
+  Proof.
+    destruct n.
+    - cbn. rewrite Z2Nat.inj_0, N2Nat.inj_0. reflexivity.
+    - rewrite N2Z.inj_pos, positive_N_nat, Z2Nat.inj_pos. reflexivity.
+  Qed.
+
+  Lemma zeros_abst : ∀ {n : N} h,
+    B.le (B.α (bv_0 n)) (zeros h (I.α (Z.of_N n))).
+  Proof.
+    intros n h.
+    unfold I.α, zeros. cbn.
+    assert (Positive : (Z.of_N n <? 0)%Z = false).
+    { destruct n; reflexivity. }
+    rewrite Positive, Nat.sub_diag.
+    destruct h; cbn.
+    - apply BP.le_top.
+    - unfold zeros_nat. rewrite N_to_nat_via_Z, N2Nat.id.
+      apply BP.le_refl.
+  Qed.
+
+  Definition ones (h : nat) (n : I.t) : B.t :=
+    match nonneg_range n with
+    | None => B.bot
+    | Some (_, None) => B.top
+    | Some (lo, Some hi) =>
+        let widths := hi - lo in
+        if h <=? widths then
+          B.top
+        else
+          fold_left (fun b w => B.join b (ones_nat w)) (seq lo (hi - lo)) (ones_nat hi)
+    end.
+
+  Lemma ones_abst : ∀ {n} h,
+    B.le (B.α (bv_not (bv_0 n))) (ones h (I.α (Z.of_N n))).
+  Proof.
+    intros n h.
+    unfold I.α, ones. cbn.
+    assert (Positive : (Z.of_N n <? 0)%Z = false).
+    { destruct n; reflexivity. }
+    rewrite Positive, Nat.sub_diag.
+    destruct h; cbn.
+    - apply BP.le_top.
+    - unfold ones_nat. rewrite N_to_nat_via_Z, N2Nat.id.
+      apply BP.le_refl.
+  Qed.
+
+  (** Number of consecutive B0 bits from the front of the list (min
+      CLZ/CTZ: first non-B0 might be 1) *)
+  Fixpoint count_leading_B0 (bits : list ubit) : nat :=
+    match bits with
+    | B0 :: rest => 1 + count_leading_B0 rest
+    | _          => 0
+    end.
+
+  (** Number of bits until the first definite B1 (max CLZ/CTZ: BU bits
+      might all be 0) *)
+  Fixpoint count_until_B1 (bits : list ubit) : nat :=
+    match bits with
+    | []        => 0
+    | B1 :: _   => 0
+    | _ :: rest => 1 + count_until_B1 rest
+    end.
+
+  Definition bits_clz_interval (bits : list ubit) : I.t :=
+    let rev_bits := rev bits in
+    let lo := Z.of_nat (count_leading_B0 rev_bits) in
+    let hi := Z.of_nat (count_until_B1 rev_bits) in
+    I.join (I.α lo) (I.α hi).
+
+  Definition count_leading_zeros (x : B.t) : I.t :=
+    match x with
+    | B.Top   => nonneg_top
+    | B.Bvs m =>
+        map_fold (λ (_ : nat) bits acc,
+          I.join (bits_clz_interval bits) acc) I.bot (`m)
+    end.
+
+  Definition bits_ctz_interval (bits : list ubit) : I.t :=
+    let lo := Z.of_nat (count_leading_B0 bits) in
+    let hi := Z.of_nat (count_until_B1 bits) in
+    I.join (I.α lo) (I.α hi).
+
+  Definition count_trailing_zeros (x : B.t) : I.t :=
+    match x with
+    | B.Top   => nonneg_top
+    | B.Bvs m =>
+        map_fold (λ (_ : nat) bits acc,
+          I.join (bits_ctz_interval bits) acc) I.bot (`m)
+    end.
+
+  Lemma zero_extend_one_width_valid (src_bits : list ubit) (dst_w : nat) :
+    length src_bits ≤ dst_w →
+    B.valid {[dst_w := src_bits ++ replicate (dst_w - length src_bits) B0]}.
+  Proof.
+    intros H. apply B.singleton_valid.
+    rewrite length_app, length_replicate. lia.
+  Qed.
+
+  (** Extend a single abstract bits list to dst_w by appending B0 padding. *)
+  Definition zero_extend_one_width (src_bits : list ubit) (dst_w : nat) : B.t :=
+    let src_w := length src_bits in
+    match decide (src_w ≤ dst_w) with
+    | left Hle =>
+        B.Bvs ({[dst_w := src_bits ++ replicate (dst_w - src_w) B0]} ↾
+               zero_extend_one_width_valid src_bits dst_w Hle)
+    | right _ => B.bot
+    end.
+
+  (** Join zero-extensions of all width entries in b to a single target width. *)
+  Definition zero_extend_to_width (b : B.t) (dst_w : nat) : B.t :=
+    match b with
+    | B.Top => B.top
+    | B.Bvs m =>
+        map_fold (λ (_ : nat) bits acc,
+          B.join (zero_extend_one_width bits dst_w) acc) B.bot (`m)
+    end.
+
+  Definition zero_extend (h : nat) (b : B.t) (n : I.t) : B.t :=
+    match nonneg_range n with
+    | None => B.bot
+    | Some (_, None) => B.top
+    | Some (lo, Some hi) =>
+        let widths := hi - lo in
+        if h <=? widths then
+          B.top
+        else
+          fold_left (fun acc w => B.join acc (zero_extend_to_width b w))
+                    (seq lo (hi - lo)) (zero_extend_to_width b hi)
+    end.
+
+  Lemma sign_extend_one_width_valid (src_bits : list ubit) (sign : ubit) (dst_w : nat) :
+    length src_bits ≤ dst_w →
+    B.valid {[dst_w := src_bits ++ replicate (dst_w - length src_bits) sign]}.
+  Proof.
+    intros H. apply B.singleton_valid.
+    rewrite length_app, length_replicate. lia.
+  Qed.
+
+  (** Extend a single abstract bits list to dst_w by replicating the MSB (sign bit). *)
+  Definition sign_extend_one_width (src_bits : list ubit) (dst_w : nat) : B.t :=
+    let src_w := length src_bits in
+    match decide (src_w ≤ dst_w) with
+    | left Hle =>
+        let sign := match rev src_bits with
+                    | s :: _ => s
+                    | []     => B0
+                    end in
+        B.Bvs ({[dst_w := src_bits ++ replicate (dst_w - src_w) sign]} ↾
+               sign_extend_one_width_valid src_bits sign dst_w Hle)
+    | right _ => B.bot
+    end.
+
+  (** Join sign-extensions of all width entries in b to a single target width. *)
+  Definition sign_extend_to_width (b : B.t) (dst_w : nat) : B.t :=
+    match b with
+    | B.Top => B.top
+    | B.Bvs m =>
+        map_fold (λ (_ : nat) bits acc,
+          B.join (sign_extend_one_width bits dst_w) acc) B.bot (`m)
+    end.
+
+  Definition sign_extend (h : nat) (b : B.t) (n : I.t) : B.t :=
+    match nonneg_range n with
+    | None => B.bot
+    | Some (_, None) => B.top
+    | Some (lo, Some hi) =>
+        let widths := hi - lo in
+        if h <=? widths then
+          B.top
+        else
+          fold_left (fun acc w => B.join acc (sign_extend_to_width b w))
+                    (seq lo (hi - lo)) (sign_extend_to_width b hi)
+    end.
+
+  Lemma bv_zero_extend_bits : ∀ {n : N} (z : N) (x : bv n),
+    (n ≤ z)%N →
+    bv_to_bits (bv_zero_extend z x) = bv_to_bits x ++ replicate (N.to_nat z - N.to_nat n) false.
+  Proof.
+    intros n z x Hnz.
+    assert (Hn_le : N.to_nat n ≤ N.to_nat z).
+    { apply N2Z.inj_le in Hnz. rewrite <- (N2Nat.id n), <- (N2Nat.id z), !nat_N_Z in Hnz. lia. }
+    apply (list_eq_same_length _ _ (N.to_nat z)).
+    - rewrite length_app, length_bv_to_bits, length_replicate. lia.
+    - rewrite length_bv_to_bits. reflexivity.
+    - intros i b1 b2 Hi L R.
+      rewrite bv_to_bits_lookup_Some in L. destruct L as [_ ->].
+      rewrite bv_zero_extend_unsigned; [| exact Hnz].
+      destruct (Nat.lt_ge_cases i (N.to_nat n)) as [Hi_lo | Hi_hi].
+      + rewrite lookup_app_l in R; [| rewrite length_bv_to_bits; exact Hi_lo].
+        rewrite bv_to_bits_lookup_Some in R. destruct R as [_ ->].
+        reflexivity.
+      + rewrite lookup_app_r in R; [| rewrite length_bv_to_bits; exact Hi_hi].
+        rewrite length_bv_to_bits in R.
+        apply lookup_replicate_1 in R. destruct R as [-> _].
+        apply bv_unsigned_spec_high.
+        rewrite <- (N2Nat.id n), nat_N_Z. lia.
+  Qed.
+
+  Lemma zero_extend_abst : ∀ {n : N} {x : bv n} {z : N} h,
+    (n ≤ z)%N →
+    B.le (B.α (bv_zero_extend z x)) (zero_extend h (B.α (bv_to_bvn x)) (I.α (Z.of_N z))).
+  Proof.
+    intros n x z h Hnz.
+    assert (Hn_le : N.to_nat n ≤ N.to_nat z).
+    { apply N2Z.inj_le in Hnz. rewrite <- (N2Nat.id n), <- (N2Nat.id z), !nat_N_Z in Hnz. lia. }
+    unfold I.α, zero_extend. cbn.
+    assert (Positive : (Z.of_N z <? 0)%Z = false) by (destruct z; reflexivity).
+    rewrite Positive, Nat.sub_diag.
+    destruct h; cbn.
+    - apply BP.le_top.
+    - rewrite N_to_nat_via_Z.
+      unfold zero_extend_to_width.
+      rewrite (B.abstract_bvs x). cbn [proj1_sig].
+      rewrite map_fold_singleton, B.join_id.
+      unfold zero_extend_one_width.
+      destruct (decide (length (map from_bool (bv_to_bits x)) ≤ N.to_nat z)) as [Hd | Hd].
+      + assert (Heq : B.α (bv_zero_extend z x) =
+                      B.Bvs ({[N.to_nat z := map from_bool (bv_to_bits x) ++
+                               replicate (N.to_nat z - length (map from_bool (bv_to_bits x))) B0]}
+                             ↾ zero_extend_one_width_valid _ _ Hd)).
+        { rewrite B.abstract_bvs. f_equal. apply subset_eq_compat.
+          rewrite bv_zero_extend_bits; [| exact Hnz].
+          rewrite map_app, fmap_replicate.
+          rewrite length_map, length_bv_to_bits. reflexivity. }
+        rewrite Heq. apply BP.le_refl.
+      + exfalso. apply Hd. rewrite (length_map from_bool), length_bv_to_bits. exact Hn_le.
+  Qed.
+
+  Lemma bv_sign_extend_bits : ∀ {n : N} (z : N) (x : bv n),
+    (n ≤ z)%N →
+    bv_to_bits (bv_sign_extend z x) =
+    bv_to_bits x ++ replicate (N.to_nat z - N.to_nat n) (hd false (rev (bv_to_bits x))).
+  Proof.
+    intros n z x Hnz.
+    assert (Hn_le : N.to_nat n ≤ N.to_nat z).
+    { apply N2Z.inj_le in Hnz. rewrite <- (N2Nat.id n), <- (N2Nat.id z), !nat_N_Z in Hnz. lia. }
+    apply (list_eq_same_length _ _ (N.to_nat z)).
+    - rewrite length_app, length_bv_to_bits, length_replicate. lia.
+    - rewrite length_bv_to_bits. reflexivity.
+    - intros i b1 b2 Hi L R.
+      rewrite bv_to_bits_lookup_Some in L. destruct L as [_ ->].
+      rewrite bv_sign_extend_unsigned.
+      destruct (Nat.lt_ge_cases i (N.to_nat n)) as [Hi_lo | Hi_hi].
+      + rewrite lookup_app_l in R; [| rewrite length_bv_to_bits; exact Hi_lo].
+        rewrite bv_to_bits_lookup_Some in R. destruct R as [_ ->].
+        rewrite bv_wrap_spec_low; [| split; [lia | rewrite <- N_nat_Z; lia]].
+        unfold bv_signed.
+        rewrite bv_swrap_spec; [| lia].
+        case_bool_decide as Hlt.
+        * reflexivity.
+        * f_equal. rewrite <- N_nat_Z in *; lia.
+      + rewrite lookup_app_r in R; [| rewrite length_bv_to_bits; exact Hi_hi].
+        rewrite length_bv_to_bits in R.
+        apply lookup_replicate_1 in R. destruct R as [-> _].
+        rewrite bv_wrap_spec_low; [| split; [lia | rewrite <- N_nat_Z; lia]].
+        unfold bv_signed.
+        rewrite bv_swrap_spec; [| lia].
+        case_bool_decide as Hlt.
+        * exfalso. rewrite <- N_nat_Z in Hlt. lia.
+        * destruct (decide (n = 0%N)) as [-> | Hn0].
+          -- assert (Hbits0 : bv_to_bits x = []).
+             { apply nil_length_inv. rewrite length_bv_to_bits. reflexivity. }
+             rewrite Hbits0. cbn.
+             apply Z.testbit_neg_r. lia.
+          -- assert (Hn0_nat : 0 < N.to_nat n).
+             { destruct n as [|p]; [contradiction |]. rewrite positive_N_nat. apply Pos2Nat.is_pos. }
+             assert (Hhd : nth 0 (rev (bv_to_bits x)) false = hd false (rev (bv_to_bits x))).
+             { destruct (rev (bv_to_bits x)); reflexivity. }
+             rewrite <- Hhd.
+             rewrite rev_nth; [| rewrite length_bv_to_bits; lia].
+             rewrite length_bv_to_bits.
+             symmetry.
+             apply nth_lookup_Some.
+             rewrite bv_to_bits_lookup_Some.
+             split; [lia | f_equal; rewrite <- N_nat_Z; lia].
+  Qed.
+
+  Lemma sign_extend_abst : ∀ {n : N} {x : bv n} {z : N} h,
+    (n ≤ z)%N →
+    B.le (B.α (bv_sign_extend z x)) (sign_extend h (B.α (bv_to_bvn x)) (I.α (Z.of_N z))).
+  Proof.
+    intros n x z h Hnz.
+    assert (Hn_le : N.to_nat n ≤ N.to_nat z).
+    { apply N2Z.inj_le in Hnz. rewrite <- (N2Nat.id n), <- (N2Nat.id z), !nat_N_Z in Hnz. lia. }
+    unfold I.α, sign_extend. cbn.
+    assert (Positive : (Z.of_N z <? 0)%Z = false) by (destruct z; reflexivity).
+    rewrite Positive, Nat.sub_diag.
+    destruct h; cbn.
+    - apply BP.le_top.
+    - rewrite N_to_nat_via_Z.
+      unfold sign_extend_to_width.
+      rewrite (B.abstract_bvs x). cbn [proj1_sig].
+      rewrite map_fold_singleton, B.join_id.
+      unfold sign_extend_one_width.
+      destruct (decide (length (map from_bool (bv_to_bits x)) ≤ N.to_nat z)) as [Hd | Hd].
+      + assert (Heq : B.α (bv_sign_extend z x) =
+                      B.Bvs ({[N.to_nat z := map from_bool (bv_to_bits x) ++
+                               replicate (N.to_nat z - length (map from_bool (bv_to_bits x)))
+                                 (match rev (map from_bool (bv_to_bits x)) with s :: _ => s | [] => B0 end)]}
+                             ↾ sign_extend_one_width_valid _ _ _ Hd)).
+        { rewrite B.abstract_bvs. f_equal. apply subset_eq_compat.
+          rewrite bv_sign_extend_bits; [| exact Hnz].
+          rewrite map_app, fmap_replicate.
+          rewrite length_map, length_bv_to_bits.
+          rewrite <- map_rev.
+          destruct (rev (bv_to_bits x)); reflexivity. }
+        rewrite Heq. apply BP.le_refl.
+      + exfalso. apply Hd. rewrite (length_map from_bool), length_bv_to_bits. exact Hn_le.
+  Qed.
+
+End Ops.
